#### 2.

​		$(1)$

​				$\begin{align}\displaystyle \int_{-a}^ax^2e^{-i\omega x}\,\mathrm dx&=\frac{1}{-i\omega}a^2(e^{-i\omega a}-e^{i\omega a})+\frac{1}{i\omega}\int_{-a}^a2xe^{-i\omega x}\,\mathrm dx \\[2mm]&=\frac{2a^2\sin\omega a}{\omega}+\frac{2}{\omega^2}a(e^{-i\omega a}+e^{i\omega a})-\frac{2}{\omega^2}\int_{-a}^ae^{-i\omega x}\,\mathrm dx\\[2mm]&=\left(\frac{2a^2}{\omega}-\frac{4}{\omega^3}\right)\sin \omega a+\frac{4a}{\omega^2}\cos \omega a\end{align}$

​		$(2)$

​				$\begin{align}\displaystyle \int_{-\infty}^{+\infty}xe^{-a|x|}e^{-i\omega x}\,\mathrm dx &=\int_{0}^{+\infty}xe^{-(a+i\omega)x}\,\mathrm dx + \int_{-\infty}^0xe^{(a-i\omega)x}\,\mathrm dx\\[2mm]&=\frac{1}{(a+i\omega)^2} -\frac{1}{(a-i\omega)^2}=-\frac{4\omega a i}{(a^2+\omega^2)^2} \end{align}$

​		$(3)$

​				$\begin{align}\displaystyle \int_{-a}^{a}e^{\mu x}e^{-i\omega x}\,\mathrm dx&=\frac{1}{\mu-i\omega}(e^{(\mu-i\omega)a}-e^{-(\mu-i\omega)a})=\frac{2\sinh(\mu-i\omega)a }{\mu-i\omega}\end{align}$

​		$(4)$

​				$\begin{align}\displaystyle \int_{-\infty}^{+\infty}\sin\lambda_0x\cdot e^{-a|x|} &e^{-i\omega x}\,\mathrm dx=-i\int_{-\infty}^{+\infty}\sin\lambda_0 x\sin\omega x e^{-a|x|}\,\mathrm dx\\[2mm]=&-\frac i2\int_{-\infty}^{+\infty}(\cos(\lambda_0+\omega)x-\cos(\lambda_0-\omega)x)e^{-a|x|}\,\mathrm dx\\[2mm]=&-\frac i2\int_{-\infty}^{+\infty}e^{i(\lambda_0+\omega)x}e^{-a|x|}-e^{i(\lambda_0-\omega)x}e^{-a|x|}\,\mathrm dx\\[2mm]=&-\frac{i}{2}\left(\frac{2a}{a^2+(\lambda_0+\omega)^2}-\frac{2a}{a^2+(\lambda_0-\omega)^2}\right)\\[2mm]=&-\frac{4 ai\lambda_0 \omega}{(a^2+(\lambda_0+\omega)^2)(a^2+(\lambda_0-\omega)^2)} \end{align}$

​		$(5)$

​				$\begin{align}\displaystyle \int_{-L}^{L}e^{i\lambda_0 x}e^{-i\omega x}\,\mathrm dx&=\frac{1}{\lambda_0 i-i\omega}(e^{(\lambda _0i-i\omega)L}-e^{-(\lambda_0i-i\omega)L})=\frac{2\sin (\lambda _0 -\omega)L }{\lambda_0-\omega}\end{align}$

​		$(6)$

​				$\begin{align}\displaystyle \int_{-\infty}^{+\infty}e^{-a x^2+ibx+c}e^{-i\omega x}\,\mathrm dx &= \int_{-\infty}^{+\infty}e^{-a(x-\frac{b-\omega}{2a}i)^2+c-\frac{(b-\omega)^2}{4a}}\,\mathrm dx\\[2mm] &=\left(\frac{\pi}{a}\right)^{\frac12} e^{-\frac{(b-\omega)^2}{4a}+c}\end{align}$
​		$(7)$

​				$\mathscr F[f] = \begin{align}\displaystyle \int_{-\infty}^{+\infty}\frac{1}{a^2+x^2}e^{-i\omega x}\,\mathrm dx\end{align}$

​				$\omega>0 $ 考虑 $(-R,R),Re^{-i\theta},\ (0\le\theta\le\pi)$ 的围道.

​				$\mathscr F[f]=\displaystyle2\pi i\Res(\frac{e^{-i\omega x}}{a^2+x^2},-ai)=\frac{\pi}{a}e^{-\omega a}$

​				$\omega<0 $ 考虑 $(-R,R),Re^{i\theta},\ (0\le\theta\le\pi)$ 的围道.

​				$\mathscr F[f]=\displaystyle2\pi i\Res(\frac{e^{-i\omega x}}{a^2+x^2},ai)=\frac{\pi}{a}e^{\omega a}$

​				$\therefore \mathscr F[f]=\displaystyle\frac{\pi}{a}e^{-|\omega|a}$

​		$(8)$

​				同上 $\omega >0$ 时 $\mathscr F[f]=\displaystyle2\pi i\Res(\frac{xe^{-i\omega x}}{a^2+x^2},-ai)=-\pi ie^{-\omega a}$

​						$\omega <0$ 时 $\mathscr F[f]=\displaystyle2\pi i\Res(\frac{xe^{-i\omega x}}{a^2+x^2},ai)=\pi ie^{\omega a}$

​						$\omega = 0$ 时 $\mathscr F[f]=0$

​		$(9)$

​				同上 $\omega>0$ 时 $\mathscr F[f]=\displaystyle2\pi i\Res(\frac{e^{-i\omega x}}{(a^2+x^2)^2},-ai)=\frac{1+\omega a}{2a^3}\pi e^{-\omega a}$

​						$\omega < 0$ 时 $\mathscr F[f]=\displaystyle2\pi i\Res(\frac{e^{-i\omega x}}{(a^2+x^2)^2},-ai)=\frac{1-\omega a}{2a^3}\pi e^{\omega a}$

​				$\therefore \mathscr F[f] = \displaystyle\frac{1+|\omega| a}{2a^3}\pi e^{-|\omega| a}$

#### 12.

​		考虑问题
$$
\left\{\begin{align}&\frac{\part^2u}{\part t^2}=a^2\frac{\part^2u}{\part x^2}+f(x,t),&-\infty<x<+\infty,t >0\\[2mm]
&u(x,0)=\varphi(x) ,\ \frac{\part }{\part t}u(x,0)=\psi(x) ,&-\infty<x<+\infty \end{align}\right.
$$
​		对$x$做$Fourier$变换

​		$U(\omega,t)=\mathscr F[u(x,t)],\ F(\omega,t)=\mathscr F[f(x,t)],\ U(\omega,0)=\Phi(\omega),\ U_t(\omega,0)=\Psi(\omega)$
$$
\left\{\begin{align}&U_{tt}(\omega,t)=-a^2\omega^2U(\omega,t)+F(\omega,t)&t >0\\[2mm]
&U(\omega,0)=\Phi(\omega) ,\ U_t(\omega,0)=\psi(\omega)  \end{align}\right.
$$
​		对$t$做$Laplace$变换

​		$U^L(\omega,p)=\mathscr L[U(\omega,t)],\ F^L(\omega,p)=\mathscr L[F(\omega,t)]$

​		$\Rightarrow\left.\begin{align}&p^2U^L(\omega,p)-U_t(\omega,0)-pU(\omega,0)=-a^2\omega^2U^L(\omega,p)+F^L(\omega,p) \end{align}\right.$

​		$\Leftrightarrow\displaystyle U^L(\omega,p)=\frac{F^L(\omega,p)+p\Phi(\omega)+\Psi(\omega)}{p^2+a^2\omega^2} $

​		对$p$做$Laplace$逆变换

​		$\Rightarrow U(\omega,t)\displaystyle=\frac1{a\omega}\int_{0}^{t}F(\omega,\tau)\sin a\omega(t-\tau)\,\mathrm d\tau+\frac{1}{a\omega}\Psi(\omega)\sin a\omega t+\Phi(\omega)\cos a\omega t$

​		对$\omega$做$Fourier$逆变换

​		$\Rightarrow\ \ \ \ \begin{align}u(x,t)=&\displaystyle\frac{1}{2}[\varphi(x+at)+\varphi(x-at)]\\&+\frac{1}{2a}\int_{x-at}^{x+at}\psi(x)\,\mathrm dx+\frac{1}{2a}\int_{0}^t\int_{x-a(t-\tau)}^{x+a(t-\tau)}f(y,\tau)\,\mathrm dy\mathrm d\tau\end{align}$



$$
\therefore\left\{\begin{align}\displaystyle&\frac{\part^2u}{\part t^2}=\frac{\part^2u}{\part x^2}+\frac{xt}{(1+x^2)^2},&-\infty<x<+\infty,t >0\\[2mm]&u(x,0)=0,\ \frac{\part }{\part t}u(x,0)=\frac{1}{1+x^2} ,&-\infty<x<+\infty \end{align}\right.
$$
​		$\begin{align}u(x,t)\displaystyle& =\frac{1}{2}\int_{x-t}^{x+t}\frac{1}{1+x^2}\,\mathrm dx+\frac{1}{2}\int_{0}^t\int_{x-t+\tau}^{x+t-\tau}\frac{y\tau}{(1+y^2)^2}\,\mathrm dy\mathrm d\tau\\[2mm]&=\frac{1}{2}[\arctan (x+t)-\arctan(x-t)]\\[2mm]&\ \ \ \ -\frac14\int_{0}^{t}\frac{\tau}{1+(x+t-\tau)^2}-\frac{\tau}{1+(x-t+\tau)^2}\,\mathrm d\tau\\[2mm]&=\frac{1}{2}[\arctan (x+t)-\arctan(x-t)]\\&\ \ \ \ -\frac14\left(\frac{1}{2}\ln\frac{1+x^2}{1+(x+t)^2}+(x+t)[\arctan(x+t)-\arctan(x)] \right)\\&\ \ \ \ +\frac14\left(\frac{1}{2}\ln\frac{1+x^2}{1+(x-t)^2}+(x-t)[\arctan(x-t)-\arctan(x)] \right)\\[2mm]&=\frac{2-x}{4}[\arctan(x+t)-\arctan(x-t)]-\frac t4[\arctan(x+t)+\arctan(x-t)]\\&\ \ \ \ +\frac t2\arctan x+\frac{1}{8}\ln\frac{1+(x+t)^2}{1+(x-t)^2}.\end{align}$

​			

​		其中 $\displaystyle \begin{align}\int_{0}^t\frac{\tau}{1+(\tau-a)^2}\mathrm d\tau&=\int_{-a}^{t-a}\frac{\tau+a}{1+\tau^2}\,\mathrm d\tau\\&=\frac12\ln\frac{1+(t-a)^2}{1+a^2}+a[\arctan(t-a)+\arctan a]\end{align}$

















#### 5.

​		$(1)$

​				$\displaystyle \int_{0}^{+\infty}\sin kt\cdot e^{-pt}\,\mathrm dt=\Im\int_{0}^{+\infty}e^{-(ki+p)t}\,\mathrm dt=\frac{k}{k^2+p^2}$

​		$(2)$

​				$I_{m}=\displaystyle \int_{0}^{+\infty}t^me^{-pt}\,\mathrm dt=\frac{m}{p}\int_{0}^{+\infty}t^{m-1}e^{-pt}\,\mathrm dt=\frac mpI_{m-1}=\frac{m!}{p^{m+1}}$

​		$(3)$

​				$\displaystyle \int_{0}^{+\infty}\frac12(\cos5t-\cos t)e^{-pt}\,\mathrm dt=\frac{p}{50+2p^2}-\frac{p}{2+p^2}$

​		$(4)$

​				$\displaystyle \int_{0}^{+\infty}\frac12(e^{\omega t}+e^{-\omega t})e^{-pt}\,\mathrm dt=\frac{p}{p^2-\omega^2}$

​		$(5)$

​				$\displaystyle \int_{0}^{+\infty}\frac12e^{-\lambda t}(e^{\omega t}-e^{-\omega t})e^{-pt}\,\mathrm dt=\frac{\omega}{(p+\lambda)^2-\omega^2}$

 #### 6.

​		$(1)$

​				$F^{(n)}(p)=\displaystyle\int_{0}^{+\infty}f(t)\cdot \frac{\mathrm d}{\mathrm dp}e^{-pt}\,\mathrm dt=\int_{0}^{+\infty}(-1)^nt^nf(t)e^{-pt}\,\mathrm dt=(-1)^n\mathscr L[t^nf(t)]$

​		$(2)$

​				$\mathscr L[e^{at}f(t)]=\displaystyle \int_{0}^{+\infty}f(t)e^{-(p-a)t}\,\mathrm dt=F(p-a),\ \mathrm{Re} (p-a)> c$





